Attempt2/Entity.dfy
@@ -8,23 +8,23 @@ module Entity {
 
   datatype Entity = Entity(
     sc: set<CNode>,
-    finputs: set<NP>,
-    foutputs: set<NP>,
-    f: map<NP, bool> --> map<NP, bool>
+    mf: MapFunction
   )
 
   opaque predicate EntitySomewhatValid(c: Circuit, e: Entity)
     requires CircuitValid(c)
   {
     && ScValid(c, e.sc)
-    && (AllPossibleOutputs(c, e.sc) >= e.foutputs >= AllOutputs(c, e.sc))
-    && (e.finputs == AllInputs(c, e.sc))
+    && (AllONPs(c, e.sc) >= e.mf.outputs >= ConnOutputs(c, e.sc))
+    && (e.mf.inputs == AllInputs(c, e.sc))
+    && (e.mf.state == AllSeq(c, e.sc))
   }
 
   lemma EntityFInputsAreValid(c: Circuit, e: Entity)
     requires CircuitValid(c)
     requires EntitySomewhatValid(c, e)
-    ensures forall np :: np in e.finputs ==> NPValid(c, np)
+    ensures forall np :: np in e.mf.inputs ==> NPValid(c, np)
+    ensures forall np :: np in StateONPs(e.mf.state) ==> NPValid(c, np)
   {
     reveal ScValid();
     reveal EntitySomewhatValid();
@@ -34,39 +34,39 @@ module Entity {
   lemma EntityFOutputsAreValid(c: Circuit, e: Entity)
     requires CircuitValid(c)
     requires EntitySomewhatValid(c, e)
-    ensures forall np :: np in e.foutputs ==> NPValid(c, np)
+    ensures forall np :: np in e.mf.outputs ==> NPValid(c, np)
+    ensures forall np :: np in StateINPs(e.mf.state) ==> NPValid(c, np)
   {
     reveal ScValid();
     reveal EntitySomewhatValid();
     reveal NPsValid();
-  }
-
-  ghost opaque predicate EntityFValid(c: Circuit, e: Entity)
-  {
-    forall knowns: map<NP, bool> :: knowns.Keys == e.finputs ==>
-      && e.f.requires(knowns)
-      && (e.f(knowns).Keys == e.foutputs)
+    assert e.mf.outputs <= AllONPs(c, e.sc);
+    reveal ONPsValid();
+    reveal AllSeq();
   }
 
   ghost opaque predicate EntityEvaluatesCorrectly(c: Circuit, e: Entity)
     requires CircuitValid(c)
     requires ScValid(c, e.sc)
-    requires EntityFValid(c, e)
+    requires MapFunctionValid(e.mf)
     requires EntitySomewhatValid(c, e)
   {
     reveal ScValid();
     EntityFOutputsAreValid(c, e);
-    reveal EntityFValid();
-    forall knowns: map<NP, bool> :: knowns.Keys == e.finputs ==>
-      forall np :: np in e.foutputs ==>
-        && Evaluate(c, np, knowns) == EvalOk(e.f(knowns)[np])
+    reveal MapFunctionValid();
+    forall fi: FI :: FIValid(fi, e.mf.inputs, e.mf.state) ==> (
+      && (forall np :: np in e.mf.outputs ==>
+          Evaluate(c, np, fi) == EvalOk(e.mf.f(fi).outputs[np]))
+      && (forall np :: np in StateINPs(e.mf.state) ==>
+          Evaluate(c, np, fi) == EvalOk(e.mf.f(fi).state[np]))
+      )
   }
 
   ghost predicate EntityValid(c: Circuit, e: Entity)
     requires CircuitValid(c)
   {
     && EntitySomewhatValid(c, e)
-    && EntityFValid(c, e)
+    && MapFunctionValid(e.mf)
     && ScValid(c, e.sc)
     && EntityEvaluatesCorrectly(c, e)
   }
@@ -74,20 +74,24 @@ module Entity {
   lemma FInputsInSc(c: Circuit, e: Entity)
     requires CircuitValid(c)
     requires EntitySomewhatValid(c, e)
-    ensures NPsInSc(e.sc, e.finputs)
+    ensures NPsInSc(e.sc, e.mf.inputs)
+    ensures NPsInSc(e.sc, StateONPs(e.mf.state))
   {
     reveal EntitySomewhatValid();
     reveal NPsInSc();
+    reveal AllSeq();
   }
 
   lemma FOutputsInSc(c: Circuit, e: Entity)
     requires CircuitValid(c)
     requires EntitySomewhatValid(c, e)
-    ensures NPsInSc(e.sc, e.foutputs)
+    ensures NPsInSc(e.sc, e.mf.outputs)
+    ensures NPsInSc(e.sc, StateINPs(e.mf.state))
   {
     reveal NPsInSc();
     reveal EntitySomewhatValid();
-    assert AllPossibleOutputs(c, e.sc) >= e.foutputs;
+    reveal AllSeq();
+    assert AllONPs(c, e.sc) >= e.mf.outputs;
   }
 
   lemma StaysInSc(c: Circuit, e: Entity, np: NP)
@@ -95,7 +99,7 @@ module Entity {
     requires EntitySomewhatValid(c, e)
     requires INPValid(c, np)
     requires np.n in e.sc
-    requires np !in e.finputs
+    requires np !in e.mf.inputs
     ensures np in c.PortSource
     ensures c.PortSource[np].n in e.sc
   {
@@ -109,26 +113,31 @@ module Entity {
     requires CircuitValid(c)
     requires ScValid(c, e.sc)
   {
-    e.foutputs >= ConnOutputs(c, e.sc)
+    e.mf.outputs >= ConnOutputs(c, e.sc)
   }
 
-  function SwapEntityF(c: Circuit, e: Entity, f: map<NP, bool> --> map<NP, bool>): (r: Entity)
+  function SwapEntityF(c: Circuit, e: Entity, mf: MapFunction): (r: Entity)
+    requires CircuitValid(c)
     requires EntityValid(c, e)
-    requires MapFunctionValid(MapFunction(e.finputs, e.foutputs, f))
+    requires mf.inputs == e.mf.inputs
+    requires mf.outputs == e.mf.outputs
+    requires mf.state == e.mf.state
+    requires MapFunctionValid(mf)
+    requires MapFunctionsEquiv(e.mf, mf)
     ensures EntityValid(c, r)
   {
     reveal EntitySomewhatValid();
-    reveal EntityFValid();
+    reveal MapFunctionValid();
     reveal ScValid();
     reveal EntityEvaluatesCorrectly();
-    Entity(e.sc, e.finputs, e.foutputs, f)
+    Entity(e.sc, mf)
   }
 
   lemma NPInFInputsOfIslandNotInPortSource(c: Circuit, e: Entity, np: NP) 
     requires CircuitValid(c)
     requires IsIsland(c, e.sc)
     requires EntityValid(c, e)
-    requires np in e.finputs
+    requires np in e.mf.inputs
     ensures np !in c.PortSource
   {
     assert np in AllInputs(c, e.sc) by {
@@ -137,18 +146,14 @@ module Entity {
     assert |ConnInputs(c, e.sc)| == 0 by {
       IsIslandNoInputs(c, e.sc);
     }
-    assert np in UnconnInputs(c, e.sc) || np in FinalInputs(c, e.sc) || np in SeqInputs(c, e.sc);
+    assert np in UnconnInputs(c, e.sc) || np in SeqInputs(c, e.sc);
     if np in UnconnInputs(c, e.sc) {
       assert np !in c.PortSource by {
         reveal UnconnInputs();
       }
     }
-    if np in FinalInputs(c, e.sc) {
-      assert ONPValid(c, np) by {
-        reveal FinalInputs();
-      }
-    }
     if np in SeqInputs(c, e.sc) {
+      reveal ONPsValid();
       assert ONPValid(c, np) by {
         reveal SeqInputs();
       }
