Attempt2/MapFunction.dfy
@@ -3,67 +3,253 @@ module MapFunction {
   import opened Circ
   import opened Utils
 
+  datatype FI = FI(
+    inputs: map<NP, bool>,
+    state: map<NP, bool>
+  )
+
+  datatype FO = FO(
+    outputs: map<NP, bool>,
+    state: map<NP, bool>
+  )
+
+  predicate FIValid(fi: FI, input_keys: set<NP>, state_keys: set<CNode>)
+  {
+    && fi.inputs.Keys == input_keys
+    && fi.state.Keys == StateONPs(state_keys)
+  }
+
+  predicate FOValid(fo: FO, output_keys: set<NP>, state_keys: set<CNode>)
+  {
+    && fo.outputs.Keys == output_keys
+    && fo.state.Keys == StateINPs(state_keys)
+  }
+
   datatype MapFunction = MapFunction(
     inputs: set<NP>,
     outputs: set<NP>,
-    f: map<NP, bool> --> map<NP, bool>
+    state: set<CNode>,
+    f: FI --> FO
   )
+
+  function StateINPs(state: set<CNode>): set<NP>
+  {
+    (set n | n in state :: NP(n, INPUT_0))
+  }
+
+  function StateONPs(state: set<CNode>): set<NP>
+  {
+    (set n | n in state :: NP(n, OUTPUT_0))
+  }
 
   ghost opaque predicate MapFunctionValid(mf: MapFunction)
   {
-    (forall x: map<NP, bool> :: x.Keys == mf.inputs ==> mf.f.requires(x)) &&
-    (forall x: map<NP, bool> :: x.Keys == mf.inputs ==> mf.f(x).Keys == mf.outputs) &&
-    SetsNoIntersection(mf.inputs, mf.outputs)
+    && (forall fi: FI :: FIValid(fi, mf.inputs, mf.state) ==> (
+        && mf.f.requires(fi)
+        && FOValid(mf.f(fi), mf.outputs, mf.state)
+    ))
+    && SetsNoIntersection(mf.inputs, mf.outputs)
+    && SetsNoIntersection(mf.outputs, StateINPs(mf.state))
+    && SetsNoIntersection(mf.inputs, StateONPs(mf.state))
   }
 
-  function GetInputs2(
-      mf1: MapFunction, mf2: MapFunction, connection: map<NP, NP>, knowns: map<NP, bool>): map<NP, bool>
-    requires MapFunctionValid(mf1)
-    requires MapFunctionValid(mf2)
-    requires forall np :: np in connection.Keys ==> np in mf2.inputs
-    requires forall np :: np in connection.Values ==> np in mf1.outputs
-    requires SetsNoIntersection(mf1.inputs + mf1.outputs, mf2.inputs + mf2.outputs)
-    requires
-        var b: set<NP> := (mf1.inputs + mf2.inputs - connection.Keys);
-        knowns.Keys == b
+  function MFLookup(mf: MapFunction, fi: FI, np: NP): bool
+    requires MapFunctionValid(mf)
+    requires FIValid(fi, mf.inputs, mf.state)
+    requires np in mf.outputs || np in StateINPs(mf.state)
   {
     reveal MapFunctionValid();
-    var inputs := mf1.inputs + mf2.inputs - connection.Keys;
-    var outputs := mf1.outputs + mf2.outputs;
-    assert forall np :: np in mf1.inputs ==> np in knowns;
-    var inputs_1 := ExtractMap(knowns, mf1.inputs);
-    var outputs_1 := mf1.f(inputs_1);
-    assert outputs_1.Keys == mf1.outputs;
-    var connected := (map np | np in connection :: np := outputs_1[connection[np]]);
+    var fo := mf.f(fi);
+    if np in mf.outputs then
+      fo.outputs[np]
+    else
+      fo.state[np]
+  }
+
+  function GetInputs2(mf1: MapFunction, mf2: MapFunction, connection: map<NP, NP>, fi: FI): map<NP, bool>
+    requires ConnectMapFunctionRequirement(mf1, mf2, connection)
+    requires FIValid(fi, mf1.inputs + (mf2.inputs - connection.Keys), mf1.state + mf2.state)
+    requires connection.Keys <= mf2.inputs
+    requires connection.Values <= mf1.outputs
+  {
+    reveal MapFunctionValid();
+    var fi_1 := ConnectFI1FromFI(mf1, mf2, connection, fi);
+    var fo_1 := mf1.f(fi_1);
+    var connected := (map np | np in connection :: np := fo_1.outputs[connection[np]]);
     assert connected.Keys == connection.Keys;
-    var combined_map := AddMaps(knowns, connected);
-    assert combined_map.Keys == mf1.inputs + mf2.inputs;
-    var inputs_2 := ExtractMap(combined_map, mf2.inputs);
+    assert fi.inputs.Keys == mf1.inputs + (mf2.inputs - connection.Keys);
+    assert connection.Keys <= mf2.inputs;
+    SubsetsNoIntersection(MFNPs(mf1), MFNPs(mf2), mf1.inputs, connection.Keys);
+    var combined_inputs := AddMaps(fi.inputs, connected);
+    assert combined_inputs.Keys == mf1.inputs + mf2.inputs;
+    var inputs_2 := ExtractMap(combined_inputs, mf2.inputs);
     inputs_2
   }
 
-  function ComposeMapFunction(
-      mf1: MapFunction, mf2: MapFunction, connection: map<NP, NP>, knowns: map<NP, bool>): map<NP, bool>
-    requires MapFunctionValid(mf1)
-    requires MapFunctionValid(mf2)
-    requires forall np :: np in connection.Keys ==> np in mf2.inputs
-    requires forall np :: np in connection.Values ==> np in mf1.outputs
-    requires SetsNoIntersection(mf1.inputs + mf1.outputs, mf2.inputs + mf2.outputs)
-    requires
-        var b: set<NP> := (mf1.inputs + mf2.inputs - connection.Keys);
-        knowns.Keys == b
+  function MFNPs(mf: MapFunction): set<NP>
   {
-    reveal MapFunctionValid();
-    assert knowns.Keys == mf1.inputs + mf2.inputs - connection.Keys;
-    ManyInThisNotInThat(connection.Keys, mf2.inputs + mf2.outputs, mf1.inputs + mf1.outputs);
-    assert forall np :: np in connection.Keys ==> np !in mf1.inputs;
-    assert forall np :: np in mf1.inputs ==> np in knowns;
-    var inputs_1 := ExtractMap(knowns, mf1.inputs);
-    var outputs_1 := mf1.f(inputs_1);
-    var inputs_2 := GetInputs2(mf1, mf2, connection, knowns);
-    var outputs_2 := mf2.f(inputs_2);
-    var combined_outputs := AddMaps(outputs_1, outputs_2);
-    combined_outputs
+    mf.inputs + mf.outputs + StateINPs(mf.state) + StateONPs(mf.state)
   }
 
+  ghost predicate ConnectMapFunctionRequirement(mf1: MapFunction, mf2: MapFunction, connection: map<NP, NP>)
+  {
+    && MapFunctionValid(mf1)
+    && MapFunctionValid(mf2)
+    && (forall np :: np in connection.Keys ==> np in mf2.inputs)
+    && (forall np :: np in connection.Values ==> np in mf1.outputs)
+    && SetsNoIntersection(MFNPs(mf1), MFNPs(mf2))
+    && SetsNoIntersection(mf1.state, mf2.state)
+  }
+
+  opaque function ConnectMapFunction(mf1: MapFunction, mf2: MapFunction, connection: map<NP, NP>): (mf: MapFunction)
+    requires ConnectMapFunctionRequirement(mf1, mf2, connection)
+    ensures MapFunctionValid(mf)
+    ensures mf.inputs == mf1.inputs + (mf2.inputs - connection.Keys)
+    ensures mf.state == mf1.state + mf2.state
+    ensures mf.outputs == mf1.outputs + mf2.outputs
+  {
+    var new_inputs := mf1.inputs + (mf2.inputs - connection.Keys);
+    var new_outputs := mf1.outputs + mf2.outputs;
+    var new_state := mf1.state + mf2.state;
+    var new_f: FI --> FO := (fi: FI) requires FIValid(fi, new_inputs, new_state) => 
+      ConnectMapFunctionF(mf1, mf2, connection, fi);
+    var mf := MapFunction(new_inputs, new_outputs, new_state, new_f);
+    assert forall fi: FI :: FIValid(fi, mf.inputs, mf.state) ==> (
+        && mf.f.requires(fi)
+        && FOValid(mf.f(fi), mf.outputs, mf.state)
+    );
+    reveal MapFunctionValid();
+    assert SetsNoIntersection(mf1.inputs, mf1.outputs);
+    assert SetsNoIntersection(mf2.inputs, mf2.outputs);
+    assert SetsNoIntersection(mf.inputs, mf.outputs);
+    assert StateINPs(mf.state) == StateINPs(mf1.state) + StateINPs(mf2.state);
+    assert StateONPs(mf.state) == StateONPs(mf1.state) + StateONPs(mf2.state);
+    assert SetsNoIntersection(mf1.inputs, StateONPs(mf1.state));
+    SubsetsNoIntersection(MFNPs(mf1), MFNPs(mf2), mf1.inputs, StateONPs(mf2.state));
+    assert SetsNoIntersection(mf1.inputs, StateONPs(mf2.state));
+    assert SetsNoIntersection(mf2.outputs, StateINPs(mf2.state));
+    SetsNoIntersectionSymm(MFNPs(mf2), MFNPs(mf1));
+    SubsetsNoIntersection(MFNPs(mf2), MFNPs(mf1), mf2.outputs, StateINPs(mf1.state));
+    assert SetsNoIntersection(mf2.outputs, StateINPs(mf1.state));
+    assert SetsNoIntersection(mf.outputs, StateINPs(mf.state));
+    assert SetsNoIntersection(mf.inputs, StateONPs(mf.state));
+    assert MapFunctionValid(mf);
+    mf
+  }
+
+  function ConnectFI1FromFI(mf1: MapFunction, mf2: MapFunction, connection: map<NP, NP>, fi: FI): (fi_1: FI)
+    requires ConnectMapFunctionRequirement(mf1, mf2, connection)
+    requires FIValid(fi, mf1.inputs + (mf2.inputs - connection.Keys), mf1.state+mf2.state)
+    ensures FIValid(fi_1, mf1.inputs, mf1.state)
+  {
+    FI(ExtractMap(fi.inputs, mf1.inputs), ExtractMap(fi.state, StateONPs(mf1.state)))
+  }
+
+  function ConnectFI2FromFI(mf1: MapFunction, mf2: MapFunction, connection: map<NP, NP>, fi: FI): (fi_2: FI)
+    requires ConnectMapFunctionRequirement(mf1, mf2, connection)
+    requires FIValid(fi, mf1.inputs + (mf2.inputs - connection.Keys), mf1.state+mf2.state)
+    ensures FIValid(fi_2, mf2.inputs, mf2.state)
+  {
+    FI(GetInputs2(mf1, mf2, connection, fi), ExtractMap(fi.state, StateONPs(mf2.state)))
+  }
+
+  lemma {:vcs_split_on_every_assert} ConnectMapFunctionMF1Preserved(mf1: MapFunction, mf2: MapFunction, connection: map<NP, NP>, fi: FI, np: NP)
+    requires ConnectMapFunctionRequirement(mf1, mf2, connection)
+    requires FIValid(fi, mf1.inputs + (mf2.inputs - connection.Keys), mf1.state+mf2.state)
+    requires np in mf1.outputs || np in StateINPs(mf1.state)
+    ensures
+      var fi_1 := ConnectFI1FromFI(mf1, mf2, connection, fi);
+      var mf := ConnectMapFunction(mf1, mf2, connection);
+      MFLookup(mf1, fi_1, np) == MFLookup(mf, fi, np)
+  {
+    var mf := ConnectMapFunction(mf1, mf2, connection);
+    var fi_1 := ConnectFI1FromFI(mf1, mf2, connection, fi);
+    var fi_2 := ConnectFI2FromFI(mf1, mf2, connection, fi);
+    reveal MapFunctionValid();
+    var fo_1 := mf1.f(fi_1);
+    var fo_2 := mf2.f(fi_2);
+    OutputsNoIntersection(mf1, mf2, connection);
+    reveal ConnectMapFunction();
+    assert mf.f(fi) == FO(AddMaps(fo_1.outputs, fo_2.outputs), AddMaps(fo_1.state, fo_2.state));
+    if np in mf1.outputs {
+      assert np in mf.outputs;
+      assert MFLookup(mf, fi, np) == fo_1.outputs[np];
+      assert MFLookup(mf1, fi_1, np) == fo_1.outputs[np];
+    } else {
+      assert np in StateINPs(mf1.state);
+      assert np in StateINPs(mf.state);
+      assert np !in mf.outputs;
+      assert MFLookup(mf, fi, np) == fo_1.state[np];
+      assert MFLookup(mf1, fi_1, np) == fo_1.state[np];
+    }
+  }
+
+  lemma ConnectMapFunctionMF2Preserved(mf1: MapFunction, mf2: MapFunction, connection: map<NP, NP>, fi: FI, np: NP)
+    requires ConnectMapFunctionRequirement(mf1, mf2, connection)
+    requires FIValid(fi, mf1.inputs + (mf2.inputs - connection.Keys), mf1.state+mf2.state)
+    requires np in mf2.outputs || np in StateINPs(mf2.state)
+    ensures
+      var fi_1 := ConnectFI1FromFI(mf1, mf2, connection, fi);
+      var fi_2 := ConnectFI2FromFI(mf1, mf2, connection, fi);
+      var mf := ConnectMapFunction(mf1, mf2, connection);
+      && MFLookup(mf2, fi_2, np) == MFLookup(mf, fi, np)
+  {
+    reveal MapFunctionValid();
+    reveal ConnectMapFunction();
+    var fi_1 := ConnectFI1FromFI(mf1, mf2, connection, fi);
+    var fi_2 := ConnectFI2FromFI(mf1, mf2, connection, fi);
+    reveal MapFunctionValid();
+    var fo_1 := mf1.f(fi_1);
+    var fo_2 := mf2.f(fi_2);
+    OutputsNoIntersection(mf1, mf2, connection);
+  }
+
+  lemma OutputsNoIntersection(mf1: MapFunction, mf2: MapFunction, connection: map<NP, NP>)
+    requires ConnectMapFunctionRequirement(mf1, mf2, connection)
+    ensures SetsNoIntersection(mf1.outputs, mf2.outputs)
+    ensures SetsNoIntersection(StateINPs(mf1.state), StateINPs(mf2.state))
+  {
+    reveal MapFunctionValid();
+    assert SetsNoIntersection(mf1.state, mf2.state);
+    assert SetsNoIntersection(mf1.outputs, mf2.outputs) by {
+      SubsetsNoIntersection(MFNPs(mf1), MFNPs(mf2), mf1.outputs, mf2.outputs);
+    }
+    assert SetsNoIntersection(StateINPs(mf1.state), StateINPs(mf2.state)) by {
+      if exists np :: np in StateINPs(mf1.state) && np in StateINPs(mf2.state) {
+        var np :| np in StateINPs(mf1.state) && np in StateINPs(mf2.state);
+        assert np.n in mf1.state;
+        assert np.n in mf2.state;
+        assert np.n in mf1.state * mf2.state;
+        assert false;
+      }
+    }
+  }
+
+  function ConnectMapFunctionF(
+      mf1: MapFunction, mf2: MapFunction, connection: map<NP, NP>, fi: FI): (fo: FO)
+    requires ConnectMapFunctionRequirement(mf1, mf2, connection)
+    requires FIValid(fi, mf1.inputs + (mf2.inputs - connection.Keys), mf1.state + mf2.state)
+    ensures FOValid(fo, mf1.outputs + mf2.outputs, mf1.state + mf2.state)
+  {
+    var fi_1 := ConnectFI1FromFI(mf1, mf2, connection, fi);
+    var fi_2 := ConnectFI2FromFI(mf1, mf2, connection, fi);
+    reveal MapFunctionValid();
+    var fo_1 := mf1.f(fi_1);
+    var fo_2 := mf2.f(fi_2);
+    OutputsNoIntersection(mf1, mf2, connection);
+    FO(AddMaps(fo_1.outputs, fo_2.outputs), AddMaps(fo_1.state, fo_2.state))
+  }
+
+  ghost predicate MapFunctionsEquiv(mf1: MapFunction, mf2: MapFunction)
+    requires MapFunctionValid(mf1)
+    requires MapFunctionValid(mf2)
+  {
+    reveal MapFunctionValid();
+    && mf1.inputs == mf2.inputs
+    && mf1.outputs == mf2.outputs
+    && mf1.state == mf2.state
+    && forall fi: FI :: FIValid(fi, mf1.inputs, mf1.state) ==> (
+      mf1.f(fi) == mf2.f(fi)
+    )
+  }
 }
