Attempt2/ConnectionEval.dfy
@@ -8,73 +8,76 @@ module ConnectionEval {
   import opened Entity
   import opened Connection
   import opened Subcircuit
+  import opened MapFunction
 
-  lemma Knowns2FromKnowns1(c: Circuit, e1: Entity, e2: Entity, connection: map<NP, NP>, knowns: map<NP, bool>, np: NP)
+  lemma Knowns2FromKnowns1(
+      c: Circuit, e1: Entity, e2: Entity, connection: map<NP, NP>, fi: FI, np: NP)
     requires ConnectEntitiesRequirements(c, e1, e2, connection)
-    requires knowns.Keys == e1.finputs + (e2.finputs - connection.Keys)
+    requires FIValid(fi, e1.mf.inputs + (e2.mf.inputs - connection.Keys), e1.mf.state + e2.mf.state)
     requires np in connection
     ensures
       && var new_c := ConnectEntitiesImpl(c, e1, e2, connection).0;
       && np in new_c.PortSource
       && var onp := new_c.PortSource[np];
-      && var knowns_1 := ExtractMap(knowns, e1.finputs);
-      && var knowns_2 := CalculateE2Inputs(c, e1, e2, connection, knowns);
+      && var fi_1 := ConnectFI1FromFI(e1.mf, e2.mf, connection, fi);
+      && var knowns_2 := GetInputs2(e1.mf, e2.mf, connection, fi);
       && (np in knowns_2)
-      && (e1.f.requires(knowns_1))
-      && (onp in e1.f(knowns_1))
-      && (knowns_2[np] == e1.f(knowns_1)[onp])
+      && (e1.mf.f.requires(fi))
+      && (onp in e1.mf.f(fi).outputs)
+      && (knowns_2[np] == e1.mf.f(fi_1).outputs[onp])
   {
     var new_c := ConnectEntitiesImpl(c, e1, e2, connection).0;
     ConnectCircuitReqFromConnectEntitiesReq(c, e1, e2, connection);
     assert new_c == ConnectCircuit(c, connection) by {
       reveal ConnectEntitiesImpl();
     }
-    var knowns_1 := ExtractMap(knowns, e1.finputs);
-    var knowns_2 := CalculateE2Inputs(c, e1, e2, connection, knowns);
+    var knowns_1 := ExtractMap(fi.inputs, e1.mf.inputs);
+    var knowns_2 := GetInputs2(e1.mf, e2.mf, connection, fi);
+    var fi_1 := ConnectFI1FromFI(e1.mf, e2.mf, connection, fi);
     var onp := connection[np];
     assert onp == new_c.PortSource[np] by {
       reveal ConnectEntitiesImpl();
       reveal ConnectionValid();
     }
-    assert np !in e1.finputs by {
+    assert np !in e1.mf.inputs by {
       ConnectionKeysInE2(c, e1, e2, connection);
       FInputsInSc(c, e1);
       reveal NPsInSc();
       SetsNoIntersectionSymm(e1.sc, e2.sc);
       InThisNotInThat(np.n, e2.sc, e1.sc);
     }
-    assert np !in knowns;
+    assert np !in fi.inputs;
 
-    var inputs_1 := ExtractMap(knowns, e1.finputs);
-    reveal EntityFValid();
-    var outputs_1 := e1.f(inputs_1);
-    assert outputs_1.Keys == e1.foutputs;
-    reveal ConnectionValid();
-    assert connection.Values <= e1.foutputs;
-    var connected := (map np | np in connection :: np := outputs_1[connection[np]]);
-    assert connected.Keys == connection.Keys;
-    assert knowns.Keys == e1.finputs + (e2.finputs - connection.Keys);
-    RearrangeKnownKeys(c, e1, e2, connection, knowns);
-    assert knowns.Keys == (e1.finputs + e2.finputs) - connection.Keys;
-    var combined_map := AddMaps(knowns, connected);
-    var inputs_2 := ExtractMap(combined_map, e2.finputs);
-    assert inputs_2 == knowns_2;
+    //var inputs_1 := ExtractMap(fi.inputs, e1.mf.inputs);
+    //reveal MapFunctionValid();
+    //var outputs_1 := e1.mf.f(FI(inputs_1, state1)).outputs;
+    //assert outputs_1.Keys == e1.mf.outputs;
+    //reveal ConnectionValid();
+    //assert connection.Values <= e1.mf.outputs;
+    //var connected := (map np | np in connection :: np := outputs_1[connection[np]]);
+    //assert connected.Keys == connection.Keys;
+    //assert knowns.Keys == e1.mf.inputs + (e2.mf.inputs - connection.Keys);
+    //RearrangeKnownKeys(c, e1, e2, connection, knowns);
+    //assert knowns.Keys == (e1.mf.inputs + e2.mf.inputs) - connection.Keys;
+    //var combined_map := AddMaps(knowns, connected);
+    //var inputs_2 := ExtractMap(combined_map, e2.mf.inputs);
+    //assert inputs_2 == knowns_2;
 
-    assert np in connected;
+    //assert np in connected;
     assert np in knowns_2;
   }
 
-  lemma ONPNotInKnownsNotInKnowns2(c: Circuit, onp: NP, e1: Entity, e2: Entity, connection: map<NP, NP>, new_c: Circuit, knowns: map<NP, bool>)
+  lemma ONPNotInKnownsNotInKnowns2(c: Circuit, onp: NP, e1: Entity, e2: Entity, connection: map<NP, NP>, new_c: Circuit, fi: FI)
     requires ConnectEntitiesRequirements(c, e1, e2, connection)
-    requires knowns.Keys == e1.finputs + (e2.finputs - connection.Keys)
+    requires FIValid(fi, e1.mf.inputs + (e2.mf.inputs - connection.Keys), e1.mf.state + e2.mf.state)
     requires new_c == ConnectEntitiesImpl(c, e1, e2, connection).0
-    requires onp !in knowns
+    requires onp !in fi.inputs
     requires ONPValid(new_c, onp)
-    ensures onp !in CalculateE2Inputs(c, e1, e2, connection, knowns)
+    ensures onp !in GetInputs2(e1.mf, e2.mf, connection, fi)
   {
-    assert onp !in e1.finputs + (e2.finputs - connection.Keys);
-    var knowns_2 := CalculateE2Inputs(c, e1, e2, connection, knowns);
-    assert knowns_2.Keys == e2.finputs;
+    assert onp !in e1.mf.inputs + (e2.mf.inputs - connection.Keys);
+    var knowns_2 := GetInputs2(e1.mf, e2.mf, connection, fi);
+    assert knowns_2.Keys == e2.mf.inputs;
     ConnectionKeysINPs(c, e1, e2, connection);
     reveal INPsValid();
   }
@@ -95,27 +98,28 @@ module ConnectionEval {
   }
 
   lemma EvaluateONPComposed1Helper(
-      c: Circuit, e1: Entity, e2: Entity, connection: map<NP, NP>, new_c: Circuit, prepath: seq<NP>, path: seq<NP>, knowns: map<NP, bool>, inp: NP)
+      c: Circuit, e1: Entity, e2: Entity, connection: map<NP, NP>, new_c: Circuit,
+      prepath: seq<NP>, path: seq<NP>, fi: FI, inp: NP)
     requires ConnectEntitiesRequirements(c, e1, e2, connection)
-    requires knowns.Keys == e1.finputs + (e2.finputs - connection.Keys)
+    requires FIValid(fi, e1.mf.inputs + (e2.mf.inputs - connection.Keys), e1.mf.state + e2.mf.state)
     requires new_c == ConnectEntitiesImpl(c, e1, e2, connection).0
     requires PathInSubcircuit(prepath, e2.sc)
     requires PathInSubcircuit(path, e1.sc)
     requires inp !in path
     requires inp.n in e1.sc
     requires INPValid(new_c, inp)
-    requires EvaluateONPUnaryBinaryRequirements(new_c, path, knowns)
-    requires EvaluateONPUnaryBinaryRequirements(new_c, prepath + path, knowns)
-    ensures forall np :: np in e1.finputs ==> np in knowns
+    requires EvaluateONPUnaryBinaryRequirements(new_c, path, fi)
+    requires EvaluateONPUnaryBinaryRequirements(new_c, prepath + path, fi)
+    ensures forall np :: np in e1.mf.inputs ==> np in fi.inputs
     ensures
       && var new_path := path + [inp];
       && Seq.HasNoDuplicates(new_path)
       && Seq.HasNoDuplicates(prepath + new_path)
       && PathValid(new_c, new_path)
       && PathValid(new_c, prepath + new_path)
-      && var knowns_1 := ExtractMap(knowns, e1.finputs);
-      && EvaluateINPInner(new_c, new_path, knowns) == EvaluateINPInner(new_c, new_path, knowns_1)
-      && Simpl(EvaluateINPInner(new_c, new_path, knowns)) == Simpl(EvaluateINPInner(new_c, prepath+new_path, knowns))
+      && var fi_1 := ConnectFI1FromFI(e1.mf, e2.mf, connection, fi);
+      && EvaluateINPInner(new_c, new_path, fi) == EvaluateINPInner(new_c, new_path, fi_1)
+      && Simpl(EvaluateINPInner(new_c, new_path, fi)) == Simpl(EvaluateINPInner(new_c, prepath+new_path, fi))
     decreases
       |NodesNotInPath(new_c, prepath + path)|, 3
   {
@@ -127,37 +131,38 @@ module ConnectionEval {
     StillHasNoDuplicates(prepath + path, inp);
     AppendPathValid(new_c, path, inp);
     AppendPathValid(new_c, prepath + path, inp);
-    assert forall np :: np in e1.finputs ==> np in knowns;
-    var knowns_1 := ExtractMap(knowns, e1.finputs);
+    assert forall np :: np in e1.mf.inputs ==> np in fi.inputs;
+    var fi_1 := ConnectFI1FromFI(e1.mf, e2.mf, connection, fi);
     var new_path := path + [inp];
     NodesNotInPathDecreases(new_c, prepath + path, inp);
     assert PathInSubcircuit(new_path, e1.sc) by {reveal PathInSubcircuit();}
     assert (prepath + path) + [inp] == prepath + (path + [inp]);
     assert Seq.Last(prepath + new_path) == inp;
-    EvaluateINPInnerComposed1(c, e1, e2, connection, new_c, prepath, new_path, knowns);
-    assert EvaluateINPInner(new_c, new_path, knowns) == EvaluateINPInner(new_c, new_path, knowns_1);
-    assert Simpl(EvaluateINPInner(new_c, new_path, knowns)) == Simpl(EvaluateINPInner(new_c, prepath+new_path, knowns));
+    EvaluateINPInnerComposed1(c, e1, e2, connection, new_c, prepath, new_path, fi);
+    assert EvaluateINPInner(new_c, new_path, fi) == EvaluateINPInner(new_c, new_path, fi_1);
+    assert Simpl(EvaluateINPInner(new_c, new_path, fi)) == Simpl(EvaluateINPInner(new_c, prepath+new_path, fi));
   }
 
   lemma EvaluateONPBinaryComposed1(
-      c: Circuit, e1: Entity, e2: Entity, connection: map<NP, NP>, new_c: Circuit, prepath: seq<NP>, path: seq<NP>, knowns: map<NP, bool>)
+      c: Circuit, e1: Entity, e2: Entity, connection: map<NP, NP>, new_c: Circuit,
+      prepath: seq<NP>, path: seq<NP>, fi: FI)
     requires ConnectEntitiesRequirements(c, e1, e2, connection)
-    requires knowns.Keys == e1.finputs + (e2.finputs - connection.Keys)
+    requires FIValid(fi, e1.mf.inputs + (e2.mf.inputs - connection.Keys), e1.mf.state + e2.mf.state)
     requires new_c == ConnectEntitiesImpl(c, e1, e2, connection).0
     requires PathInSubcircuit(prepath, e2.sc)
     requires PathInSubcircuit(path, e1.sc)
-    requires EvaluateONPBinaryRequirements(new_c, path, knowns)
-    requires EvaluateONPBinaryRequirements(new_c, prepath + path, knowns)
+    requires EvaluateONPBinaryRequirements(new_c, path, fi)
+    requires EvaluateONPBinaryRequirements(new_c, prepath + path, fi)
     ensures
-      (forall np :: np in e1.finputs ==> np in knowns) &&
-      var knowns_1 := ExtractMap(knowns, e1.finputs);
+      (forall np :: np in e1.mf.inputs ==> np in fi.inputs) &&
+      var fi_1 := ConnectFI1FromFI(e1.mf, e2.mf, connection, fi);
       var np := Seq.Last(path);
-      && (EvaluateONPBinary(new_c, path, knowns) == EvaluateONPBinary(new_c, path, knowns_1))
-      && (Simpl(EvaluateONPBinary(new_c, path, knowns)) == Simpl(EvaluateONPBinary(new_c, prepath+path, knowns)))
+      && (EvaluateONPBinary(new_c, path, fi) == EvaluateONPBinary(new_c, path, fi_1))
+      && (Simpl(EvaluateONPBinary(new_c, path, fi)) == Simpl(EvaluateONPBinary(new_c, prepath+path, fi)))
     decreases |NodesNotInPath(new_c, prepath + path)|, 4
   {
-    assert forall np :: np in e1.finputs ==> np in knowns;
-    var knowns_1 := ExtractMap(knowns, e1.finputs);
+    assert forall np :: np in e1.mf.inputs ==> np in fi.inputs;
+    var fi_1 := ConnectFI1FromFI(e1.mf, e2.mf, connection, fi);
     var head := Seq.Last(path);
     assert head == Seq.Last(prepath + path);
     assert head.n in e1.sc by {reveal PathInSubcircuit();}
@@ -168,61 +173,61 @@ module ConnectionEval {
     NPNotInPathHelper(inp_0, e1.sc, e2.sc, prepath, path);
     NPNotInPathHelper(inp_1, e1.sc, e2.sc, prepath, path);
     if inp_0 in path {
-      assert (EvaluateONPBinary(new_c, path, knowns) == EvaluateONPBinary(new_c, path, knowns_1));
-      assert (Simpl(EvaluateONPBinary(new_c, path, knowns)) == Simpl(EvaluateONPBinary(new_c, prepath+path, knowns)));
+      assert (EvaluateONPBinary(new_c, path, fi) == EvaluateONPBinary(new_c, path, fi_1));
+      assert (Simpl(EvaluateONPBinary(new_c, path, fi)) == Simpl(EvaluateONPBinary(new_c, prepath+path, fi)));
     } else if inp_1 in path {
-      assert (EvaluateONPBinary(new_c, path, knowns) == EvaluateONPBinary(new_c, path, knowns_1));
-      assert (Simpl(EvaluateONPBinary(new_c, path, knowns)) == Simpl(EvaluateONPBinary(new_c, prepath+path, knowns)));
+      assert (EvaluateONPBinary(new_c, path, fi) == EvaluateONPBinary(new_c, path, fi_1));
+      assert (Simpl(EvaluateONPBinary(new_c, path, fi)) == Simpl(EvaluateONPBinary(new_c, prepath+path, fi)));
     } else {
-      EvaluateONPComposed1Helper(c, e1, e2, connection, new_c, prepath, path, knowns, inp_0);
-      EvaluateONPComposed1Helper(c, e1, e2, connection, new_c, prepath, path, knowns, inp_1);
+      EvaluateONPComposed1Helper(c, e1, e2, connection, new_c, prepath, path, fi, inp_0);
+      EvaluateONPComposed1Helper(c, e1, e2, connection, new_c, prepath, path, fi, inp_1);
 
       assert prepath + (path + [inp_0]) == (prepath + path) + [inp_0];
       assert prepath + (path + [inp_1]) == (prepath + path) + [inp_1];
 
-      assert (Simpl(EvaluateONPBinary(new_c, path, knowns)) == Simpl(EvaluateONPBinary(new_c, prepath+path, knowns)));
+      assert (Simpl(EvaluateONPBinary(new_c, path, fi)) == Simpl(EvaluateONPBinary(new_c, prepath+path, fi)));
     }
   }
 
   lemma EvaluateONPComposed2Helper(
-      c: Circuit, e1: Entity, e2: Entity, connection: map<NP, NP>, new_c: Circuit, path: seq<NP>, knowns: map<NP, bool>, inp: NP)
+      c: Circuit, e1: Entity, e2: Entity, connection: map<NP, NP>, new_c: Circuit, path: seq<NP>, fi: FI, inp: NP)
     requires ConnectEntitiesRequirements(c, e1, e2, connection)
-    requires knowns.Keys == e1.finputs + (e2.finputs - connection.Keys)
+    requires FIValid(fi, e1.mf.inputs + (e2.mf.inputs - connection.Keys), e1.mf.state + e2.mf.state)
     requires new_c == ConnectEntitiesImpl(c, e1, e2, connection).0
     requires PathInSubcircuit(path, e2.sc)
-    requires EvaluateONPUnaryBinaryRequirements(new_c, path, knowns)
+    requires EvaluateONPUnaryBinaryRequirements(new_c, path, fi)
     requires INPValid(new_c, inp)
     requires inp !in path
     requires inp.n in e2.sc
     ensures
-      var knowns_2 := CalculateE2Inputs(c, e1, e2, connection, knowns);
+      var fi_2 := ConnectFI2FromFI(e1.mf, e2.mf, connection, fi);
       var new_path := path + [inp];
       Seq.HasNoDuplicates(new_path) &&
       PathValid(new_c, new_path) &&
-      (EvaluateINPInner(new_c, new_path, knowns) == EvaluateINPInner(new_c, new_path, knowns_2))
+      (EvaluateINPInner(new_c, new_path, fi) == EvaluateINPInner(new_c, new_path, fi_2))
     decreases |NodesNotInPath(new_c, path)|, 4
   {
     StillHasNoDuplicates(path, inp);
     AppendPathValid(new_c, path, inp);
-    var knowns_2 := CalculateE2Inputs(c, e1, e2, connection, knowns);
     var new_path := path + [inp];
     NodesNotInPathDecreases(new_c, path, inp);
     reveal PathInSubcircuit();
-    EvaluateINPInnerComposed2(c, e1, e2, connection, new_c, new_path, knowns);
-    assert (EvaluateINPInner(new_c, new_path, knowns) == EvaluateINPInner(new_c, new_path, knowns_2));
+    EvaluateINPInnerComposed2(c, e1, e2, connection, new_c, new_path, fi);
+    var fi_2 := ConnectFI2FromFI(e1.mf, e2.mf, connection, fi);
+    assert (EvaluateINPInner(new_c, new_path, fi) == EvaluateINPInner(new_c, new_path, fi_2));
   }
 
   lemma EvaluateONPBinaryComposed2(
-      c: Circuit, e1: Entity, e2: Entity, connection: map<NP, NP>, new_c: Circuit, path: seq<NP>, knowns: map<NP, bool>)
+      c: Circuit, e1: Entity, e2: Entity, connection: map<NP, NP>, new_c: Circuit, path: seq<NP>, fi: FI)
     requires ConnectEntitiesRequirements(c, e1, e2, connection)
-    requires knowns.Keys == e1.finputs + (e2.finputs - connection.Keys)
+    requires FIValid(fi, e1.mf.inputs + (e2.mf.inputs - connection.Keys), e1.mf.state + e2.mf.state)
     requires new_c == ConnectEntitiesImpl(c, e1, e2, connection).0
     requires PathInSubcircuit(path, e2.sc)
-    requires EvaluateONPBinaryRequirements(new_c, path, knowns)
+    requires EvaluateONPBinaryRequirements(new_c, path, fi)
     ensures
-      var knowns_2 := CalculateE2Inputs(c, e1, e2, connection, knowns);
-      (Seq.Last(path) !in knowns_2) &&
-      (EvaluateONPBinary(new_c, path, knowns) == EvaluateONPBinary(new_c, path, knowns_2))
+      var fi_2 := ConnectFI2FromFI(e1.mf, e2.mf, connection, fi);
+      (Seq.Last(path) !in fi_2.inputs) &&
+      (EvaluateONPBinary(new_c, path, fi) == EvaluateONPBinary(new_c, path, fi_2))
     decreases |NodesNotInPath(new_c, path)|, 5
   {
     var head := Seq.Last(path);
@@ -234,57 +239,57 @@ module ConnectionEval {
     var inp_0 := NP(head.n, INPUT_0);
     var inp_1 := NP(head.n, INPUT_1);
     assert INPValid(new_c, inp_0) && INPValid(new_c, inp_1) by {reveal CircuitValid();}
-    var knowns_2 := CalculateE2Inputs(c, e1, e2, connection, knowns);
-    assert head !in knowns;
-    ONPNotInKnownsNotInKnowns2(c, head, e1, e2, connection, new_c, knowns);
-    assert head !in knowns_2;
+    var fi_2 := ConnectFI2FromFI(e1.mf, e2.mf, connection, fi);
+    assert head !in fi_2.inputs;
+    ONPNotInKnownsNotInKnowns2(c, head, e1, e2, connection, new_c, fi);
     if inp_0 in path {
-      assert (EvaluateONPBinary(new_c, path, knowns) == EvaluateONPBinary(new_c, path, knowns_2));
+      assert (EvaluateONPBinary(new_c, path, fi) == EvaluateONPBinary(new_c, path, fi_2));
     } else if inp_1 in path {
-      assert (EvaluateONPBinary(new_c, path, knowns) == EvaluateONPBinary(new_c, path, knowns_2));
+      assert (EvaluateONPBinary(new_c, path, fi) == EvaluateONPBinary(new_c, path, fi_2));
     } else {
       assert 
         var new_path := path + [inp_0];
         && Seq.HasNoDuplicates(new_path)
         && PathValid(new_c, new_path)
-        && (EvaluateINPInner(new_c, new_path, knowns) == EvaluateINPInner(new_c, new_path, knowns_2)) by {
+        && (EvaluateINPInner(new_c, new_path, fi) == EvaluateINPInner(new_c, new_path, fi_2)) by {
           //AppendPathValid(new_path, inp_0);
-          EvaluateONPComposed2Helper(c, e1, e2, connection, new_c, path, knowns, inp_0);
+          EvaluateONPComposed2Helper(c, e1, e2, connection, new_c, path, fi, inp_0);
         }
       assert 
         var new_path := path + [inp_1];
         && Seq.HasNoDuplicates(new_path)
         && PathValid(new_c, new_path)
-        && (EvaluateINPInner(new_c, new_path, knowns) == EvaluateINPInner(new_c, new_path, knowns_2)) by {
+        && (EvaluateINPInner(new_c, new_path, fi) == EvaluateINPInner(new_c, new_path, fi_2)) by {
           //AppendPathValid(new_path, inp_0);
-          EvaluateONPComposed2Helper(c, e1, e2, connection, new_c, path, knowns, inp_1);
+          EvaluateONPComposed2Helper(c, e1, e2, connection, new_c, path, fi, inp_1);
         }
-      assert EvaluateONPBinary(new_c, path, knowns) == EvaluateONPBinary(new_c, path, knowns_2);
+      assert EvaluateONPBinary(new_c, path, fi) == EvaluateONPBinary(new_c, path, fi_2);
     }
     assert
-      var knowns_2 := CalculateE2Inputs(c, e1, e2, connection, knowns);
-      (EvaluateONPBinary(new_c, path, knowns) == EvaluateONPBinary(new_c, path, knowns_2));
+      var knowns_2 := GetInputs2(e1.mf, e2.mf, connection, fi);
+      (EvaluateONPBinary(new_c, path, fi) == EvaluateONPBinary(new_c, path, fi_2));
   }
 
   lemma EvaluateONPUnaryComposed1(
-      c: Circuit, e1: Entity, e2: Entity, connection: map<NP, NP>, new_c: Circuit, prepath: seq<NP>, path: seq<NP>, knowns: map<NP, bool>)
+      c: Circuit, e1: Entity, e2: Entity, connection: map<NP, NP>, new_c: Circuit,
+      prepath: seq<NP>, path: seq<NP>, fi: FI)
     requires ConnectEntitiesRequirements(c, e1, e2, connection)
-    requires knowns.Keys == e1.finputs + (e2.finputs - connection.Keys)
+    requires FIValid(fi, e1.mf.inputs + (e2.mf.inputs - connection.Keys), e1.mf.state + e2.mf.state)
     requires new_c == ConnectEntitiesImpl(c, e1, e2, connection).0
     requires PathInSubcircuit(prepath, e2.sc)
     requires PathInSubcircuit(path, e1.sc)
-    requires EvaluateONPUnaryRequirements(new_c, path, knowns)
-    requires EvaluateONPUnaryRequirements(new_c, prepath+path, knowns)
+    requires EvaluateONPUnaryRequirements(new_c, path, fi)
+    requires EvaluateONPUnaryRequirements(new_c, prepath+path, fi)
     ensures
-      (forall np :: np in e1.finputs ==> np in knowns) &&
-      var knowns_1 := ExtractMap(knowns, e1.finputs);
+      (forall np :: np in e1.mf.inputs ==> np in fi.inputs) &&
+      var fi_1 := ConnectFI1FromFI(e1.mf, e2.mf, connection, fi);
       var np := Seq.Last(path);
-      (EvaluateONPUnary(new_c, path, knowns) == EvaluateONPUnary(new_c, path, knowns_1)) &&
-      (Simpl(EvaluateONPUnary(new_c, path, knowns)) == Simpl(EvaluateONPUnary(new_c, prepath+path, knowns)))
+      (EvaluateONPUnary(new_c, path, fi) == EvaluateONPUnary(new_c, path, fi_1)) &&
+      (Simpl(EvaluateONPUnary(new_c, path, fi)) == Simpl(EvaluateONPUnary(new_c, prepath+path, fi)))
     decreases |NodesNotInPath(new_c, prepath + path)|, 5
   {
-    assert forall np :: np in e1.finputs ==> np in knowns;
-    var knowns_1 := ExtractMap(knowns, e1.finputs);
+    assert forall np :: np in e1.mf.inputs ==> np in fi.inputs;
+    var fi_1 := ConnectFI1FromFI(e1.mf, e2.mf, connection, fi);
     var head := Seq.Last(path);
     assert head == Seq.Last(prepath + path);
     assert head.n in e1.sc by {reveal PathInSubcircuit();}
@@ -293,31 +298,31 @@ module ConnectionEval {
     assert INPValid(new_c, inp_0) by {reveal CircuitValid();}
     NPNotInPathHelper(inp_0, e1.sc, e2.sc, prepath, path);
     if inp_0 in path {
-      assert (EvaluateONPUnary(new_c, path, knowns) == EvaluateONPUnary(new_c, path, knowns_1));
-      assert (Simpl(EvaluateONPUnary(new_c, path, knowns)) == Simpl(EvaluateONPUnary(new_c, prepath+path, knowns)));
+      assert (EvaluateONPUnary(new_c, path, fi) == EvaluateONPUnary(new_c, path, fi_1));
+      assert (Simpl(EvaluateONPUnary(new_c, path, fi)) == Simpl(EvaluateONPUnary(new_c, prepath+path, fi)));
     } else {
-      EvaluateONPComposed1Helper(c, e1, e2, connection, new_c, prepath, path, knowns, inp_0);
+      EvaluateONPComposed1Helper(c, e1, e2, connection, new_c, prepath, path, fi, inp_0);
       assert prepath + (path + [inp_0]) == (prepath + path) + [inp_0];
-      assert (Simpl(EvaluateONPUnary(new_c, path, knowns)) == Simpl(EvaluateONPUnary(new_c, prepath+path, knowns)));
+      assert (Simpl(EvaluateONPUnary(new_c, path, fi)) == Simpl(EvaluateONPUnary(new_c, prepath+path, fi)));
     }
   }
 
   lemma EvaluateONPUnaryComposed2(
-      c: Circuit, e1: Entity, e2: Entity, connection: map<NP, NP>, new_c: Circuit, path: seq<NP>, knowns: map<NP, bool>)
+      c: Circuit, e1: Entity, e2: Entity, connection: map<NP, NP>, new_c: Circuit, path: seq<NP>, fi: FI)
     requires ConnectEntitiesRequirements(c, e1, e2, connection)
-    requires knowns.Keys == e1.finputs + (e2.finputs - connection.Keys)
+    requires FIValid(fi, e1.mf.inputs + (e2.mf.inputs - connection.Keys), e1.mf.state + e2.mf.state)
     requires new_c == ConnectEntitiesImpl(c, e1, e2, connection).0
     requires PathInSubcircuit(path, e2.sc)
-    requires EvaluateONPUnaryRequirements(new_c, path, knowns)
+    requires EvaluateONPUnaryRequirements(new_c, path, fi)
     ensures
-      var knowns_2 := CalculateE2Inputs(c, e1, e2, connection, knowns);
-      (Seq.Last(path) !in knowns_2) &&
-      EvaluateONPUnary(new_c, path, knowns) == EvaluateONPUnary(new_c, path, knowns_2)
+      var fi_2 := ConnectFI2FromFI(e1.mf, e2.mf, connection, fi);
+      (Seq.Last(path) !in fi_2.inputs) &&
+      EvaluateONPUnary(new_c, path, fi) == EvaluateONPUnary(new_c, path, fi_2)
     decreases |NodesNotInPath(new_c, path)|, 4
   {
     var head := Seq.Last(path);
-    assert head !in knowns;
-    ONPNotInKnownsNotInKnowns2(c, head, e1, e2, connection, new_c, knowns);
+    assert head !in fi.inputs;
+    ONPNotInKnownsNotInKnowns2(c, head, e1, e2, connection, new_c, fi);
     var inp_0 := NP(head.n, INPUT_0);
     if inp_0 in path {
     } else {
@@ -326,7 +331,7 @@ module ConnectionEval {
       assert PathInSubcircuit(path + [inp_0], e2.sc) by {
         reveal PathInSubcircuit();
       }
-      EvaluateINPInnerComposed2(c, e1, e2, connection, new_c, path + [inp_0], knowns);
+      EvaluateINPInnerComposed2(c, e1, e2, connection, new_c, path + [inp_0], fi);
     }
   }
 
@@ -341,26 +346,28 @@ module ConnectionEval {
     reveal Seq.HasNoDuplicates();
   }
 
-  lemma EvaluateINPInnerComposed1(c: Circuit, e1: Entity, e2: Entity, connection: map<NP, NP>, new_c: Circuit, prepath: seq<NP>, path: seq<NP>, knowns: map<NP, bool>)
+  lemma EvaluateINPInnerComposed1(
+      c: Circuit, e1: Entity, e2: Entity, connection: map<NP, NP>, new_c: Circuit,
+      prepath: seq<NP>, path: seq<NP>, fi: FI)
     requires ConnectEntitiesRequirements(c, e1, e2, connection)
-    requires knowns.Keys == e1.finputs + (e2.finputs - connection.Keys)
+    requires FIValid(fi, e1.mf.inputs + (e2.mf.inputs - connection.Keys), e1.mf.state + e2.mf.state)
     requires new_c == ConnectEntitiesImpl(c, e1, e2, connection).0
     requires PathInSubcircuit(path, e1.sc)
     requires PathInSubcircuit(prepath, e2.sc)
-    requires EvaluateINPInnerRequirements(new_c, path, knowns)
-    requires EvaluateINPInnerRequirements(new_c, prepath + path, knowns)
+    requires EvaluateINPInnerRequirements(new_c, path)
+    requires EvaluateINPInnerRequirements(new_c, prepath + path)
     ensures
-      var knowns_1 := ExtractMap(knowns, e1.finputs);
-      (EvaluateINPInner(new_c, path, knowns) == EvaluateINPInner(new_c, path, knowns_1)) &&
-      (Simpl(EvaluateINPInner(new_c, path, knowns)) == Simpl(EvaluateINPInner(new_c, prepath+path, knowns)))
+      var fi_1 := ConnectFI1FromFI(e1.mf, e2.mf, connection, fi);
+      (EvaluateINPInner(new_c, path, fi) == EvaluateINPInner(new_c, path, fi_1)) &&
+      (Simpl(EvaluateINPInner(new_c, path, fi)) == Simpl(EvaluateINPInner(new_c, prepath+path, fi)))
     decreases |NodesNotInPath(new_c, prepath + path)|, 2
   {
     ConnectEntitiesEntitiesStillValid(c, e1, e2, connection);
     assert new_c == ConnectCircuit(c, connection) by {
       reveal ConnectEntitiesImpl();
     }
-    
-    var knowns_1 := ExtractMap(knowns, e1.finputs); var np := Seq.Last(path);
+    var fi_1 := ConnectFI1FromFI(e1.mf, e2.mf, connection, fi);
+    var np := Seq.Last(path);
     assert np.n in e1.sc by {
       reveal PathInSubcircuit();
     }
@@ -368,40 +375,39 @@ module ConnectionEval {
     assert Seq.HasNoDuplicates(path);
     HasNoDuplicatesMeansHeadNotInTail(path);
     assert np !in tail;
-    if np in e1.finputs {
-      assert np in knowns;
-      assert np in knowns_1;
-      assert EvaluateINPInner(new_c, path, knowns) == EvaluateINPInner(new_c, path, knowns_1);
-      assert Simpl(EvaluateINPInner(new_c, path, knowns)) == Simpl(EvaluateINPInner(new_c, prepath+path, knowns));
+    if np in e1.mf.inputs {
+      assert np in fi.inputs;
+      assert np in fi_1.inputs;
+      assert EvaluateINPInner(new_c, path, fi) == EvaluateINPInner(new_c, path, fi_1);
+      assert Simpl(EvaluateINPInner(new_c, path, fi)) == Simpl(EvaluateINPInner(new_c, prepath+path, fi));
     } else {
-      assert np !in knowns by {
-        assert knowns.Keys == e1.finputs + (e2.finputs - connection.Keys);
+      assert np !in fi.inputs by {
+        assert fi.inputs.Keys == e1.mf.inputs + (e2.mf.inputs - connection.Keys);
         InThisNotInThat(np.n, e1.sc, e2.sc);
         assert np.n !in e2.sc;
         FInputsInSc(new_c, e2);
         reveal NPsInSc();
-        assert np !in e2.finputs;
+        assert np !in e2.mf.inputs;
       }
-      assert np !in knowns_1;
+      assert np !in fi_1.inputs;
       if np in new_c.PortSource {
         var onp := new_c.PortSource[np];
         assert ONPValid(new_c, onp) by {
           reveal CircuitValid();
         }
         assert onp.n in e1.sc by {
-          assert np !in e1.finputs;
+          assert np !in e1.mf.inputs;
           reveal EntitySomewhatValid();
           assert np !in AllInputs(new_c, e1.sc);
           assert np !in ConnInputs(new_c, e1.sc);
           reveal ConnInputs();
         }
-        assert EvaluateINPInnerRequirements(new_c, path, knowns);
-        assert EvaluateINPInnerRequirements(new_c, path, knowns_1);
-        assert EvaluateINPInnerRequirements(new_c, prepath + path, knowns);
+        assert EvaluateINPInnerRequirements(new_c, path);
+        assert EvaluateINPInnerRequirements(new_c, prepath + path);
         if onp in path {
-          assert EvaluateINPInner(new_c, path, knowns) == EvalError({}, {path + [onp]});
-          assert EvaluateINPInner(new_c, path, knowns) == EvaluateINPInner(new_c, path, knowns_1);
-          assert Simpl(EvaluateINPInner(new_c, path, knowns)) == Simpl(EvaluateINPInner(new_c, prepath+path, knowns));
+          assert EvaluateINPInner(new_c, path, fi) == EvalError({}, {path + [onp]});
+          assert EvaluateINPInner(new_c, path, fi) == EvaluateINPInner(new_c, path, fi_1);
+          assert Simpl(EvaluateINPInner(new_c, path, fi)) == Simpl(EvaluateINPInner(new_c, prepath+path, fi));
         } else {
           assert NPValid(new_c, onp) by {
             reveal CircuitValid();
@@ -418,32 +424,34 @@ module ConnectionEval {
           assert PathInSubcircuit(path + [onp], e1.sc) by {
             reveal PathInSubcircuit();
           }
-          EvaluateONPInnerComposed1(c, e1, e2, connection, new_c, prepath, path + [onp], knowns);
-          assert EvaluateINPInner(new_c, path, knowns) == EvaluateINPInner(new_c, path, knowns_1);
-          assert Simpl(EvaluateINPInner(new_c, path, knowns)) == Simpl(EvaluateINPInner(new_c, prepath+path, knowns));
+          EvaluateONPInnerComposed1(c, e1, e2, connection, new_c, prepath, path + [onp], fi);
+          assert EvaluateINPInner(new_c, path, fi) == EvaluateINPInner(new_c, path, fi_1);
+          assert Simpl(EvaluateINPInner(new_c, path, fi)) == Simpl(EvaluateINPInner(new_c, prepath+path, fi));
         }
       } else {
-        assert EvaluateINPInner(new_c, path, knowns) == EvaluateINPInner(new_c, path, knowns_1);
-        assert Simpl(EvaluateINPInner(new_c, path, knowns)) == Simpl(EvaluateINPInner(new_c, prepath+path, knowns));
+        assert EvaluateINPInner(new_c, path, fi) == EvaluateINPInner(new_c, path, fi_1);
+        assert Simpl(EvaluateINPInner(new_c, path, fi)) == Simpl(EvaluateINPInner(new_c, prepath+path, fi));
       }
     }
   }
 
-  lemma EvaluateINPInnerComposed2(c: Circuit, e1: Entity, e2: Entity, connection: map<NP, NP>, new_c: Circuit, path: seq<NP>, knowns: map<NP, bool>)
+  lemma EvaluateINPInnerComposed2(
+      c: Circuit, e1: Entity, e2: Entity, connection: map<NP, NP>, new_c: Circuit,
+      path: seq<NP>, fi: FI)
     requires ConnectEntitiesRequirements(c, e1, e2, connection)
-    requires knowns.Keys == e1.finputs + (e2.finputs - connection.Keys)
+    requires FIValid(fi, e1.mf.inputs + (e2.mf.inputs - connection.Keys), e1.mf.state + e2.mf.state)
     requires new_c == ConnectEntitiesImpl(c, e1, e2, connection).0
     requires PathInSubcircuit(path, e2.sc)
-    requires EvaluateINPInnerRequirements(new_c, path, knowns)
+    requires EvaluateINPInnerRequirements(new_c, path)
     ensures
-      var knowns_2 := CalculateE2Inputs(c, e1, e2, connection, knowns);
-      (EvaluateINPInner(new_c, path, knowns) == EvaluateINPInner(new_c, path, knowns_2))
+      var fi_2 := ConnectFI2FromFI(e1.mf, e2.mf, connection, fi);
+      (EvaluateINPInner(new_c, path, fi) == EvaluateINPInner(new_c, path, fi_2))
     decreases |NodesNotInPath(new_c, path)|, 2
   {
     ConnectEntitiesEntitiesStillValid(c, e1, e2, connection);
-    assert forall np :: np in e1.finputs ==> np in knowns;
-    var knowns_1 := ExtractMap(knowns, e1.finputs);
-    var knowns_2 := CalculateE2Inputs(c, e1, e2, connection, knowns);
+    assert forall np :: np in e1.mf.inputs ==> np in fi.inputs;
+    var fi_1 := ConnectFI1FromFI(e1.mf, e2.mf, connection, fi);
+    var fi_2 := ConnectFI2FromFI(e1.mf, e2.mf, connection, fi);
     var np := Seq.Last(path);
     assert np.n in e2.sc by {
       reveal PathInSubcircuit();
@@ -452,9 +460,9 @@ module ConnectionEval {
     assert Seq.HasNoDuplicates(path);
     HasNoDuplicatesMeansHeadNotInTail(path);
     assert np !in tail;
-    if np in e2.finputs {
-      if np in knowns {
-        assert EvaluateINPInner(new_c, path, knowns) == EvaluateINPInner(new_c, path, knowns_2);
+    if np in e2.mf.inputs {
+      if np in fi.inputs {
+        assert EvaluateINPInner(new_c, path, fi) == EvaluateINPInner(new_c, path, fi_2);
       } else {
         assert np in connection.Keys;
         assert (np in new_c.PortSource) by {
@@ -462,7 +470,7 @@ module ConnectionEval {
           reveal ConnectEntitiesImpl();
         }
         var onp := new_c.PortSource[np];
-        assert onp.n in e1.sc && onp in e1.foutputs by {
+        assert onp.n in e1.sc && onp in e1.mf.outputs by {
           reveal ConnectEntitiesImpl();
           reveal ConnectionValid();
           assert onp in connection.Values;
@@ -481,30 +489,30 @@ module ConnectionEval {
         LengthOneNoDuplicates([onp]);
         assert PathValid(new_c, [onp]) by {reveal PathValid();}
         assert PathInSubcircuit([onp], e1.sc) by {reveal PathInSubcircuit();}
-        EvaluateONPInnerComposed1(c, e1, e2, connection, new_c, path, [onp], knowns);
-        assert (EvaluateONPInner(new_c, [onp], knowns) == EvaluateONPInner(new_c, [onp], knowns_1)); //  (1)
-        assert (Simpl(EvaluateONPInner(new_c, path + [onp], knowns)) == Simpl(EvaluateONPInner(new_c, [onp], knowns))); // (2)
-        assert EvaluateINPInner(new_c, path, knowns) == EvaluateONPInner(new_c, path + [onp], knowns); // (3)
-        assert (e1.f.requires(knowns_1)) && (e1.f(knowns_1).Keys == e1.foutputs) && (knowns_2[np] == e1.f(knowns_1)[onp]) by { // (4)
-          Knowns2FromKnowns1(c, e1, e2, connection, knowns, np);
-          reveal EntityFValid();
+        EvaluateONPInnerComposed1(c, e1, e2, connection, new_c, path, [onp], fi);
+        assert (EvaluateONPInner(new_c, [onp], fi) == EvaluateONPInner(new_c, [onp], fi_1)); //  (1)
+        assert (Simpl(EvaluateONPInner(new_c, path + [onp], fi)) == Simpl(EvaluateONPInner(new_c, [onp], fi))); // (2)
+        assert EvaluateINPInner(new_c, path, fi) == EvaluateONPInner(new_c, path + [onp], fi); // (3)
+        assert (e1.mf.f.requires(fi_1)) && (e1.mf.f(fi_1).outputs.Keys == e1.mf.outputs) && (fi_2.inputs[np] == e1.mf.f(fi_1).outputs[onp]) by { // (4)
+          Knowns2FromKnowns1(c, e1, e2, connection, fi, np);
+          reveal MapFunctionValid();
         }
-        assert EvaluateONPInner(new_c, [onp], knowns_1) == EvalOk(e1.f(knowns_1)[onp]) by {
+        assert EvaluateONPInner(new_c, [onp], fi_1) == EvalOk(e1.mf.f(fi_1).outputs[onp]) by {
           assert EntityValid(new_c, e1);
           reveal EntityEvaluatesCorrectly();
         }
-        Knowns2FromKnowns1(c, e1, e2, connection, knowns, np);
-        assert EvaluateINPInner(new_c, path, knowns_2) == EvalOk(knowns_2[np]); // by it's own def
-        assert EvaluateINPInner(new_c, path, knowns_2) == EvaluateONPInner(new_c, [onp], knowns_1); // by (4) and (5)
-        assert EvaluateINPInner(new_c, path, knowns_2) == EvaluateONPInner(new_c, [onp], knowns); // by (1)
-        assert EvaluateINPInner(new_c, path, knowns_2) == EvaluateONPInner(new_c, path + [onp], knowns); // by (2)
-        assert EvaluateINPInner(new_c, path, knowns_2) == EvaluateINPInner(new_c, path, knowns); // by (3)
+        Knowns2FromKnowns1(c, e1, e2, connection, fi, np);
+        assert EvaluateINPInner(new_c, path, fi_2) == EvalOk(fi_2.inputs[np]); // by it's own def
+        assert EvaluateINPInner(new_c, path, fi_2) == EvaluateONPInner(new_c, [onp], fi_1); // by (4) and (5)
+        assert EvaluateINPInner(new_c, path, fi_2) == EvaluateONPInner(new_c, [onp], fi); // by (1)
+        assert EvaluateINPInner(new_c, path, fi_2) == EvaluateONPInner(new_c, path + [onp], fi); // by (2)
+        assert EvaluateINPInner(new_c, path, fi_2) == EvaluateINPInner(new_c, path, fi); // by (3)
       }
     } else {
-      assert np !in e2.finputs;
-      assert knowns_2.Keys == e2.finputs;
-      assert np !in knowns_2;
-      assert np !in knowns by {
+      assert np !in e2.mf.inputs;
+      assert fi_2.inputs.Keys == e2.mf.inputs;
+      assert np !in fi_2.inputs;
+      assert np !in fi.inputs by {
         assert np.n in e2.sc;
         SetsNoIntersectionSymm(e1.sc, e2.sc);
         InThisNotInThat(np.n, e2.sc, e1.sc);
@@ -518,47 +526,49 @@ module ConnectionEval {
           reveal CircuitValid();
         }
         assert onp.n in e2.sc by {
-          assert np !in e2.finputs;
+          assert np !in e2.mf.inputs;
           reveal EntitySomewhatValid();
           assert np !in AllInputs(new_c, e2.sc);
           assert np !in ConnInputs(new_c, e2.sc);
           reveal ConnInputs();
         }
         if onp in path {
-          assert EvaluateINPInner(new_c, path, knowns) == EvaluateINPInner(new_c, path, knowns_2);
+          assert EvaluateINPInner(new_c, path, fi) == EvaluateINPInner(new_c, path, fi_2);
         } else {
           NodesNotInPathDecreases(new_c, path, onp);
           StillHasNoDuplicates(path, onp);
           assert PathInSubcircuit(path + [onp], e2.sc) by {
             reveal PathInSubcircuit();
           }
-          EvaluateONPInnerComposed2(c, e1, e2, connection, new_c, path + [onp], knowns);
-          assert EvaluateINPInner(new_c, path, knowns) == EvaluateINPInner(new_c, path, knowns_2);
+          EvaluateONPInnerComposed2(c, e1, e2, connection, new_c, path + [onp], fi);
+          assert EvaluateINPInner(new_c, path, fi) == EvaluateINPInner(new_c, path, fi_2);
         }
       } else {
-        assert EvaluateINPInner(new_c, path, knowns) == EvaluateINPInner(new_c, path, knowns_2);
+        assert EvaluateINPInner(new_c, path, fi) == EvaluateINPInner(new_c, path, fi_2);
       }
     }
   }
 
-  lemma EvaluateONPInnerComposed1(c: Circuit, e1: Entity, e2: Entity, connection: map<NP, NP>, new_c: Circuit, prepath: seq<NP>, path: seq<NP>, knowns: map<NP, bool>)
+  lemma EvaluateONPInnerComposed1(
+      c: Circuit, e1: Entity, e2: Entity, connection: map<NP, NP>, new_c: Circuit,
+      prepath: seq<NP>, path: seq<NP>, fi: FI)
     requires ConnectEntitiesRequirements(c, e1, e2, connection)
-    requires knowns.Keys == e1.finputs + (e2.finputs - connection.Keys)
+    requires FIValid(fi, e1.mf.inputs + (e2.mf.inputs - connection.Keys), e1.mf.state + e2.mf.state)
     requires new_c == ConnectEntitiesImpl(c, e1, e2, connection).0
-    requires EvaluateONPInnerRequirements(new_c, prepath + path, knowns)
-    requires EvaluateONPInnerRequirements(new_c, path, knowns)
+    requires EvaluateONPInnerRequirements(new_c, prepath + path)
+    requires EvaluateONPInnerRequirements(new_c, path)
     requires PathInSubcircuit(path, e1.sc)
     requires PathInSubcircuit(prepath, e2.sc)
     ensures
-      (forall np :: np in e1.finputs ==> np in knowns) &&
-      var knowns_1 := ExtractMap(knowns, e1.finputs);
-      (EvaluateONPInner(new_c, path, knowns) == EvaluateONPInner(new_c, path, knowns_1)) &&
-      (Simpl(EvaluateONPInner(new_c, prepath + path, knowns)) == Simpl(EvaluateONPInner(new_c, path, knowns)))
+      (forall np :: np in e1.mf.inputs ==> np in fi.inputs) &&
+      var fi_1 := ConnectFI1FromFI(e1.mf, e2.mf, connection, fi);
+      (EvaluateONPInner(new_c, path, fi) == EvaluateONPInner(new_c, path, fi_1)) &&
+      (Simpl(EvaluateONPInner(new_c, prepath + path, fi)) == Simpl(EvaluateONPInner(new_c, path, fi)))
     decreases |NodesNotInPath(new_c, prepath + path)|, 6
   {
     ConnectEntitiesEntitiesStillValid(c, e1, e2, connection);
-    assert forall np :: np in e1.finputs ==> np in knowns;
-    var knowns_1 := ExtractMap(knowns, e1.finputs);
+    assert forall np :: np in e1.mf.inputs ==> np in fi.inputs;
+    var fi_1 := ConnectFI1FromFI(e1.mf, e2.mf, connection, fi);
     var np := Seq.Last(path);
     assert (np.n in e1.sc) && (np.n !in e2.sc) by {
       reveal PathInSubcircuit();
@@ -566,14 +576,14 @@ module ConnectionEval {
     }
     Seq.LemmaAppendLast(prepath, path);
     assert np == Seq.Last(prepath + path);
-    if np in knowns {
-      assert np in knowns_1 by {
+    if np in fi.inputs {
+      assert np in fi_1.inputs by {
         FInputsInSc(new_c, e2);
         reveal NPsInSc();
-        assert np !in e2.finputs;
+        assert np !in e2.mf.inputs;
       }
-      assert EvaluateONPInner(new_c, path, knowns) == EvaluateONPInner(new_c, path, knowns_1);
-      assert Simpl(EvaluateONPInner(new_c, prepath + path, knowns)) == Simpl(EvaluateONPInner(new_c, path, knowns));
+      assert EvaluateONPInner(new_c, path, fi) == EvaluateONPInner(new_c, path, fi_1);
+      assert Simpl(EvaluateONPInner(new_c, prepath + path, fi)) == Simpl(EvaluateONPInner(new_c, path, fi));
     } else {
       assert np.n in new_c.NodeKind by {
         reveal CircuitValid();
@@ -581,112 +591,112 @@ module ConnectionEval {
       var nk := new_c.NodeKind[np.n];
       match nk
         case CXor() => {
-          EvaluateONPBinaryComposed1(c, e1, e2, connection, new_c, prepath, path, knowns);
+          EvaluateONPBinaryComposed1(c, e1, e2, connection, new_c, prepath, path, fi);
         }
         case CAnd() => {
-          EvaluateONPBinaryComposed1(c, e1, e2, connection, new_c, prepath, path, knowns);
+          EvaluateONPBinaryComposed1(c, e1, e2, connection, new_c, prepath, path, fi);
         }
         case CInv() => {
-          EvaluateONPUnaryComposed1(c, e1, e2, connection, new_c, prepath, path, knowns);
+          EvaluateONPUnaryComposed1(c, e1, e2, connection, new_c, prepath, path, fi);
         }
         case CConst(b) => {}
-        case CInput() => {}
         case CSeq() => {}
-      assert EvaluateONPInner(new_c, path, knowns) == EvaluateONPInner(new_c, path, knowns_1);
-      assert Simpl(EvaluateONPInner(new_c, prepath + path, knowns)) == Simpl(EvaluateONPInner(new_c, path, knowns));
+      assert EvaluateONPInner(new_c, path, fi) == EvaluateONPInner(new_c, path, fi_1);
+      assert Simpl(EvaluateONPInner(new_c, prepath + path, fi)) == Simpl(EvaluateONPInner(new_c, path, fi));
     }
-    assert EvaluateONPInner(new_c, path, knowns) == EvaluateONPInner(new_c, path, knowns_1);
-    assert Simpl(EvaluateONPInner(new_c, prepath + path, knowns)) == Simpl(EvaluateONPInner(new_c, path, knowns));
+    assert EvaluateONPInner(new_c, path, fi) == EvaluateONPInner(new_c, path, fi_1);
+    assert Simpl(EvaluateONPInner(new_c, prepath + path, fi)) == Simpl(EvaluateONPInner(new_c, path, fi));
   }
 
-  lemma EvaluateONPInnerComposed2(c: Circuit, e1: Entity, e2: Entity, connection: map<NP, NP>, new_c: Circuit, path: seq<NP>, knowns: map<NP, bool>)
+  lemma EvaluateONPInnerComposed2(
+      c: Circuit, e1: Entity, e2: Entity, connection: map<NP, NP>, new_c: Circuit,
+      path: seq<NP>, fi: FI)
     requires ConnectEntitiesRequirements(c, e1, e2, connection)
-    requires knowns.Keys == e1.finputs + (e2.finputs - connection.Keys)
+    requires FIValid(fi, e1.mf.inputs + (e2.mf.inputs - connection.Keys), e1.mf.state + e2.mf.state)
     requires new_c == ConnectEntitiesImpl(c, e1, e2, connection).0
-    requires EvaluateONPInnerRequirements(new_c, path, knowns)
+    requires EvaluateONPInnerRequirements(new_c, path)
     requires PathInSubcircuit(path, e2.sc)
     ensures
-      var knowns_2 := CalculateE2Inputs(c, e1, e2, connection, knowns);
+      var fi_2 := ConnectFI2FromFI(e1.mf, e2.mf, connection, fi);
       var np := Seq.Last(path);
-      (EvaluateONPInner(new_c, path, knowns) == EvaluateONPInner(new_c, path, knowns_2))
+      (EvaluateONPInner(new_c, path, fi) == EvaluateONPInner(new_c, path, fi_2))
     decreases |NodesNotInPath(new_c, path)|, 6
   {
     ConnectEntitiesEntitiesStillValid(c, e1, e2, connection);
-    var knowns_2 := CalculateE2Inputs(c, e1, e2, connection, knowns);
+    var fi_2 := ConnectFI2FromFI(e1.mf, e2.mf, connection, fi);
     var np := Seq.Last(path);
     assert (np.n in e2.sc) && (np.n !in e1.sc) by {
       reveal PathInSubcircuit();
       SetsNoIntersectionSymm(e2.sc, e1.sc);
       InThisNotInThat(np.n, e2.sc, e1.sc);
     }
-    if np in knowns {
-      assert np in knowns_2 by {
+    if np in fi.inputs {
+      assert np in fi_2.inputs by {
         assert np.n in e2.sc;
         FInputsInSc(new_c, e1);
         reveal NPsInSc();
         SetsNoIntersectionSymm(e2.sc, e1.sc);
         InThisNotInThat(np.n, e2.sc, e1.sc);
-        assert np !in e1.finputs;
+        assert np !in e1.mf.inputs;
       }
-      assert EvaluateONPInner(new_c, path, knowns) == EvaluateONPInner(new_c, path, knowns_2);
+      assert EvaluateONPInner(new_c, path, fi) == EvaluateONPInner(new_c, path, fi_2);
     } else {
-      assert np !in e2.finputs by {
+      assert np !in e2.mf.inputs by {
         ConnectionKeysINPs(c, e1, e2, connection);
         assert ONPValid(new_c, np);
         NotBothINPValidONPValid(new_c, np);
         reveal INPsValid();
       }
       var nk := new_c.NodeKind[np.n];
-      assert !nk.CInput? && !nk.CSeq? by {
-        if (nk.CInput? || nk.CSeq?) {
-          reveal FinalInputs();
+      assert !nk.CSeq? by {
+        if nk.CSeq? {
           reveal SeqInputs();
           assert np.n in e2.sc;
           assert ONPValid(new_c, np);
           assert nk.CSeq? ==> np in SeqInputs(new_c, e2.sc);
-          assert nk.CInput? ==> np in FinalInputs(new_c, e2.sc);
-          assert np in FinalInputs(new_c, e2.sc) + SeqInputs(new_c, e2.sc);
+          assert np in SeqInputs(new_c, e2.sc);
           reveal EntitySomewhatValid();
-          assert e2.finputs == AllInputs(new_c, e2.sc);
-          assert np in e2.finputs;
+          assert e2.mf.inputs == AllInputs(new_c, e2.sc);
+          assert np in e2.mf.inputs;
         }
       }
       match nk
         case CXor() => {
-          EvaluateONPBinaryComposed2(c, e1, e2, connection, new_c, path, knowns);
-      assert EvaluateONPInner(new_c, path, knowns) == EvaluateONPInner(new_c, path, knowns_2);
+          EvaluateONPBinaryComposed2(c, e1, e2, connection, new_c, path, fi);
+      assert EvaluateONPInner(new_c, path, fi) == EvaluateONPInner(new_c, path, fi_2);
         }
         case CAnd() => {
-          EvaluateONPBinaryComposed2(c, e1, e2, connection, new_c, path, knowns);
-      assert EvaluateONPInner(new_c, path, knowns) == EvaluateONPInner(new_c, path, knowns_2);
+          EvaluateONPBinaryComposed2(c, e1, e2, connection, new_c, path, fi);
+      assert EvaluateONPInner(new_c, path, fi) == EvaluateONPInner(new_c, path, fi_2);
         }
         case CInv() => {
-          EvaluateONPUnaryComposed2(c, e1, e2, connection, new_c, path, knowns);
-      assert EvaluateONPInner(new_c, path, knowns) == EvaluateONPInner(new_c, path, knowns_2);
+          EvaluateONPUnaryComposed2(c, e1, e2, connection, new_c, path, fi);
+      assert EvaluateONPInner(new_c, path, fi) == EvaluateONPInner(new_c, path, fi_2);
         }
         case CConst(b) => {
-      assert EvaluateONPInner(new_c, path, knowns) == EvaluateONPInner(new_c, path, knowns_2);
+      assert EvaluateONPInner(new_c, path, fi) == EvaluateONPInner(new_c, path, fi_2);
 
         }
-        case CInput() => {}
         case CSeq() => {}
-      assert EvaluateONPInner(new_c, path, knowns) == EvaluateONPInner(new_c, path, knowns_2);
+      assert EvaluateONPInner(new_c, path, fi) == EvaluateONPInner(new_c, path, fi_2);
     }
   }
 
-  lemma EvaluateConnectEntitiesInner(c: Circuit, e1: Entity, e2: Entity, connection: map<NP, NP>, new_c: Circuit, np: NP, knowns: map<NP, bool>)
+  lemma EvaluateConnectEntitiesInner(
+      c: Circuit, e1: Entity, e2: Entity, connection: map<NP, NP>,
+      new_c: Circuit, np: NP, fi: FI)
     requires ConnectEntitiesRequirements(c, e1, e2, connection)
-    requires knowns.Keys == e1.finputs + (e2.finputs - connection.Keys)
+    requires FIValid(fi, e1.mf.inputs + (e2.mf.inputs - connection.Keys), e1.mf.state + e2.mf.state)
     requires new_c == ConnectEntitiesImpl(c, e1, e2, connection).0
     requires NPValid(new_c, np)
-    requires np in e1.foutputs || np in e2.foutputs
+    requires np in e1.mf.outputs || np in e2.mf.outputs || np in StateINPs(e1.mf.state + e2.mf.state)
     ensures
       var (new_c, e) := ConnectEntitiesImpl(c, e1, e2, connection);
-      var knowns_1 := ExtractMap(knowns, e1.finputs);
-      var knowns_2 := CalculateE2Inputs(c, e1, e2, connection, knowns);
+      var fi_1 := ConnectFI1FromFI(e1.mf, e2.mf, connection, fi);
+      var fi_2 := ConnectFI2FromFI(e1.mf, e2.mf, connection, fi);
       && NPValid(new_c, np)
-      && (np.n in e1.sc ==> Evaluate(new_c, np, knowns_1) == Evaluate(new_c, np, knowns))
-      && (np.n in e2.sc ==> Evaluate(new_c, np, knowns_2) == Evaluate(new_c, np, knowns))
+      && (np.n in e1.sc ==> Evaluate(new_c, np, fi_1) == Evaluate(new_c, np, fi))
+      && (np.n in e2.sc ==> Evaluate(new_c, np, fi_2) == Evaluate(new_c, np, fi))
   {
     ConnectEntitiesEntitiesStillValid(c, e1, e2, connection);
     var prepath: seq<NP> := [];
@@ -696,9 +706,9 @@ module ConnectionEval {
       reveal PathValid();
     }
 
-    assert forall np :: np in e1.finputs ==> np in knowns;
-    var knowns_1 := ExtractMap(knowns, e1.finputs);
-    var knowns_2 := CalculateE2Inputs(c, e1, e2, connection, knowns);
+    assert forall np :: np in e1.mf.inputs ==> np in fi.inputs;
+    var fi_1 := ConnectFI1FromFI(e1.mf, e2.mf, connection, fi);
+    var fi_2 := ConnectFI2FromFI(e1.mf, e2.mf, connection, fi);
 
     LengthOneNoDuplicates(path);
     LengthOneNoDuplicates(prepath + path);
@@ -708,54 +718,64 @@ module ConnectionEval {
     } else {
       FOutputsInSc(new_c, e1);
       reveal NPsInSc();
-      assert np !in e1.foutputs;
-      assert np in e2.foutputs;
+      assert np !in e1.mf.outputs;
+      assert np in e2.mf.outputs;
       FOutputsInSc(new_c, e2);
       assert PathInSubcircuit(path, e2.sc) by { reveal PathInSubcircuit(); }
     }
 
     if ONPValid(new_c, np) {
       if np.n in e1.sc {
-        EvaluateONPInnerComposed1(c, e1, e2, connection, new_c, prepath, path, knowns);
-        assert EvaluateONPInner(new_c, path, knowns) == EvaluateONPInner(new_c, path, knowns_1);
+        EvaluateONPInnerComposed1(c, e1, e2, connection, new_c, prepath, path, fi);
+        assert EvaluateONPInner(new_c, path, fi) == EvaluateONPInner(new_c, path, fi_1);
       } else {
-        EvaluateONPInnerComposed2(c, e1, e2, connection, new_c, path, knowns);
-        assert EvaluateONPInner(new_c, path, knowns) == EvaluateONPInner(new_c, path, knowns_2);
+        EvaluateONPInnerComposed2(c, e1, e2, connection, new_c, path, fi);
+        assert EvaluateONPInner(new_c, path, fi) == EvaluateONPInner(new_c, path, fi_2);
       }
     } else {
       if np.n in e1.sc {
-        EvaluateINPInnerComposed1(c, e1, e2, connection, new_c, prepath, path, knowns);
-        assert EvaluateINPInner(new_c, path, knowns) == EvaluateINPInner(new_c, path, knowns_1);
+        EvaluateINPInnerComposed1(c, e1, e2, connection, new_c, prepath, path, fi);
+        assert EvaluateINPInner(new_c, path, fi) == EvaluateINPInner(new_c, path, fi_1);
       } else {
-        EvaluateINPInnerComposed2(c, e1, e2, connection, new_c, path, knowns);
-        assert EvaluateINPInner(new_c, path, knowns) == EvaluateINPInner(new_c, path, knowns_2);
+        EvaluateINPInnerComposed2(c, e1, e2, connection, new_c, path, fi);
+        assert EvaluateINPInner(new_c, path, fi) == EvaluateINPInner(new_c, path, fi_2);
       }
     }
     if np.n in e1.sc {
       InThisNotInThat(np.n, e1.sc, e2.sc);
       assert np.n !in e2.sc;
-      assert Evaluate(new_c, np, knowns) == Evaluate(new_c, np, knowns_1);
+      assert Evaluate(new_c, np, fi) == Evaluate(new_c, np, fi_1);
     } else {
       assert np.n in e2.sc;
-      assert Evaluate(new_c, np, knowns) == Evaluate(new_c, np, knowns_2);
+      assert Evaluate(new_c, np, fi) == Evaluate(new_c, np, fi_2);
     }
   }
 
-  lemma EvaluateConnectEntities(c: Circuit, e1: Entity, e2: Entity, connection: map<NP, NP>, new_c: Circuit, np: NP, knowns: map<NP, bool>)
+  lemma {:vcs_split_on_every_assert} EvaluateConnectEntities(
+      c: Circuit, e1: Entity, e2: Entity, connection: map<NP, NP>, new_c: Circuit, np: NP, fi: FI)
     requires ConnectEntitiesRequirements(c, e1, e2, connection)
-    requires knowns.Keys == e1.finputs + (e2.finputs - connection.Keys)
+    requires FIValid(fi, e1.mf.inputs + (e2.mf.inputs - connection.Keys), e1.mf.state + e2.mf.state)
     requires new_c == ConnectEntitiesImpl(c, e1, e2, connection).0
     requires NPValid(new_c, np)
-    requires np in e1.foutputs || np in e2.foutputs
+    requires np in e1.mf.outputs || np in e2.mf.outputs || np in StateINPs(e1.mf.state + e2.mf.state)
     ensures
       var (new_c, e) := ConnectEntitiesImpl(c, e1, e2, connection);
-      && e.f.requires(knowns)
-      && np in e.f(knowns)
+      && e.mf.f.requires(fi)
       && NPValid(new_c, np)
-      && Evaluate(new_c, np, knowns) == EvalOk(e.f(knowns)[np])
+      && (np in (e1.mf.outputs + e2.mf.outputs) ==>
+          && np in e.mf.f(fi).outputs
+          && Evaluate(new_c, np, fi) == EvalOk(e.mf.f(fi).outputs[np]))
+      && (np in StateINPs(e1.mf.state + e2.mf.state) ==>
+          && np in e.mf.f(fi).state
+          && Evaluate(new_c, np, fi) == EvalOk(e.mf.f(fi).state[np]))
   {
-    EvaluateConnectEntitiesInner(c, e1, e2, connection, new_c, np, knowns);
+    EvaluateConnectEntitiesInner(c, e1, e2, connection, new_c, np, fi);
     var (new_c, e) := ConnectEntitiesImpl(c, e1, e2, connection);
+    assert e.mf.f.requires(fi) by {
+      assert e.mf.inputs == e1.mf.inputs + (e2.mf.inputs - connection.Keys);
+      reveal MapFunctionValid();
+      reveal ConnectEntitiesImpl();
+    }
     ConnectEntitiesSomewhatValid(c, e1, e2, connection);
     assert ScValid(new_c, e1.sc) && ScValid(new_c, e2.sc) by {
       reveal EntitySomewhatValid();
@@ -766,65 +786,90 @@ module ConnectionEval {
     assert EntityValid(new_c, e1);
     assert EntityValid(new_c, e2);
 
-    var knowns_1 := ExtractMap(knowns, e1.finputs);
-    var knowns_2 := CalculateE2Inputs(c, e1, e2, connection, knowns);
+    var fi_1 := ConnectFI1FromFI(e1.mf, e2.mf, connection, fi);
+    var fi_2 := ConnectFI2FromFI(e1.mf, e2.mf, connection, fi);
 
-    assert e.foutputs == e1.foutputs + e2.foutputs by {
+    assert e.mf.outputs == e1.mf.outputs + e2.mf.outputs by {
       reveal ConnectEntitiesImpl();
     }
     EntityFOutputsAreValid(new_c, e);
     FOutputsInSc(c, e1);
-    if np in e1.foutputs {
+    if np in e1.mf.outputs || np in StateINPs(e1.mf.state) {
       reveal NPsInSc();
       assert np.n in e1.sc;
-      assert Evaluate(new_c, np, knowns_1) == Evaluate(new_c, np, knowns);
-      reveal EntityFValid();
-      assert knowns_1.Keys == e1.finputs;
-      assert e1.f(knowns_1).Keys == e1.foutputs;
-      assert Evaluate(new_c, np, knowns_1) == EvalOk(e1.f(knowns_1)[np]) by {
-        assert EntityEvaluatesCorrectly(c, e1);
-        reveal EntityEvaluatesCorrectly();
+      assert Evaluate(new_c, np, fi_1) == Evaluate(new_c, np, fi);
+      reveal MapFunctionValid();
+      assert fi_1.inputs.Keys == e1.mf.inputs;
+      assert e1.mf.f(fi_1).outputs.Keys == e1.mf.outputs;
+      if np in e1.mf.outputs {
+        assert Evaluate(new_c, np, fi_1) == EvalOk(e1.mf.f(fi_1).outputs[np]) by {
+          assert EntityEvaluatesCorrectly(c, e1);
+          reveal EntityEvaluatesCorrectly();
+        }
+      } else {
+        assert Evaluate(new_c, np, fi_1) == EvalOk(e1.mf.f(fi_1).state[np]) by {
+          assert EntityEvaluatesCorrectly(c, e1);
+          reveal EntityEvaluatesCorrectly();
+        }
       }
-      assert Evaluate(new_c, np, knowns) == Evaluate(new_c, np, knowns_1);
-      assert np in e.foutputs by {
+      assert Evaluate(new_c, np, fi) == Evaluate(new_c, np, fi_1);
+      assert np in e.mf.outputs || np in StateINPs(e.mf.state) by {
         reveal ConnectEntitiesImpl();
       }
-      assert knowns.Keys == e.finputs by {
+      assert fi.inputs.Keys == e.mf.inputs by {
         reveal ConnectEntitiesImpl();
       }
       ConnectEntitiesFValid(c, e1, e2, connection);
-      assert EntityFValid(new_c, e);
-      assert e.f.requires(knowns);
-      assert EvalOk(e1.f(knowns_1)[np]) == EvalOk(e.f(knowns)[np]) by {
-        reveal ConnectEntitiesImpl();
-        assert np in e.foutputs;
-        assert np in e.f(knowns);
+      assert MapFunctionValid(e.mf);
+      assert e.mf.f.requires(fi);
+      if np in e1.mf.outputs {
+        assert EvalOk(e1.mf.f(fi_1).outputs[np]) == EvalOk(e.mf.f(fi).outputs[np]) by {
+          reveal ConnectEntitiesImpl();
+          assert np in e.mf.outputs;
+          assert np in e.mf.f(fi).outputs;
+        }
+      } else {
+        assert EvalOk(e1.mf.f(fi_1).state[np]) == EvalOk(e.mf.f(fi).state[np]) by {
+          reveal ConnectEntitiesImpl();
+          assert np in e.mf.outputs;
+          assert np in e.mf.f(fi).state;
+        }
       }
-      assert Evaluate(new_c, np, knowns) == EvalOk(e.f(knowns)[np]);
+      assert Evaluate(new_c, np, fi) == EvalOk(e.mf.f(fi).outputs[np]);
     } else {
-      assert np in e2.foutputs;
-      assert np in e.foutputs by {
+      assert np in e2.mf.outputs || np in StateINPs(e2.mf.state);
+      assert np in e.mf.outputs || np in StateINPs(e.mf.state) by {
         reveal ConnectEntitiesImpl();
       }
       ConnectEntitiesFValid(c, e1, e2, connection);
-      reveal EntityFValid();
+      reveal MapFunctionValid();
       reveal ConnectEntitiesImpl();
-      assert knowns.Keys == e.finputs;
-      assert e.f.requires(knowns);
-      assert e.f(knowns).Keys == e.foutputs;
+      assert fi.inputs.Keys == e.mf.inputs;
+      assert e.mf.f.requires(fi);
+      assert e.mf.f(fi).outputs.Keys == e.mf.outputs;
       FOutputsInSc(new_c, e2);
       reveal NPsInSc();
       assert np.n in e2.sc;
       reveal EntityEvaluatesCorrectly();
-      assert Evaluate(new_c, np, knowns_2) == EvalOk(e2.f(knowns_2)[np]);
-      ConnectEntitiesFHelper(c, e1, e2, connection, knowns, np);
-      assert EvalOk(e2.f(knowns_2)[np]) == EvalOk(e.f(knowns)[np]) by {
-        reveal ConnectEntitiesImpl();
+      if np in e2.mf.outputs {
+        assert Evaluate(new_c, np, fi_2) == EvalOk(e2.mf.f(fi_2).outputs[np]);
+        ConnectEntitiesFHelper(c, e1, e2, connection, fi, np);
+        assert EvalOk(e2.mf.f(fi_2).outputs[np]) == EvalOk(e.mf.f(fi).outputs[np]) by {
+          reveal ConnectEntitiesImpl();
+        }
+        assert Evaluate(new_c, np, fi) == Evaluate(new_c, np, fi_2);
+        assert EvalOk(e2.mf.f(fi_2).outputs[np]) == EvalOk(e.mf.f(fi).outputs[np]);
+        assert Evaluate(new_c, np, fi) == EvalOk(e.mf.f(fi).outputs[np]);
+      } else {
+        assert Evaluate(new_c, np, fi_2) == EvalOk(e2.mf.f(fi_2).state[np]);
+        ConnectEntitiesFHelper(c, e1, e2, connection, fi, np);
+        assert EvalOk(e2.mf.f(fi_2).outputs[np]) == EvalOk(e.mf.f(fi).state[np]) by {
+          reveal ConnectEntitiesImpl();
+        }
+        assert Evaluate(new_c, np, fi) == Evaluate(new_c, np, fi_2);
+        assert EvalOk(e2.mf.f(fi_2).outputs[np]) == EvalOk(e.mf.f(fi).state[np]);
+        assert Evaluate(new_c, np, fi) == EvalOk(e.mf.f(fi).state[np]);
       }
-      assert Evaluate(new_c, np, knowns) == Evaluate(new_c, np, knowns_2);
-      assert EvalOk(e2.f(knowns_2)[np]) == EvalOk(e.f(knowns)[np]);
-      assert Evaluate(new_c, np, knowns) == EvalOk(e.f(knowns)[np]);
-
     }
   }
 
@@ -837,36 +882,54 @@ module ConnectionEval {
     var (new_c, e) := ConnectEntitiesImpl(c, e1, e2, connection);
     ConnectEntitiesFValid(c, e1, e2, connection);
     ConnectEntitiesSomewhatValid(c, e1, e2, connection);
-    assert e.foutputs == e1.foutputs + e2.foutputs by {
+    assert e.mf.outputs == e1.mf.outputs + e2.mf.outputs by {
       reveal ConnectEntitiesImpl();
     }
-    assert e.finputs == e1.finputs + (e2.finputs-connection.Keys) by {
+    assert e.mf.inputs == e1.mf.inputs + (e2.mf.inputs-connection.Keys) by {
       reveal ConnectEntitiesImpl();
     }
-    forall knowns: map<NP, bool> | (knowns.Keys == e.finputs)
-      ensures e.f.requires(knowns)
-      ensures forall np :: np in e.foutputs ==>
-          np in e.f(knowns) &&
+    assert e.mf.state == e1.mf.state + e2.mf.state by {
+      reveal ConnectEntitiesImpl();
+    }
+    forall fi: FI | FIValid(fi, e.mf.inputs, e.mf.state)
+      ensures e.mf.f.requires(fi)
+      ensures forall np :: np in e.mf.outputs ==>
+          np in e.mf.f(fi).outputs &&
           NPValid(new_c, np) &&
-          (Evaluate(new_c, np, knowns) == EvalOk(e.f(knowns)[np]))
+          (Evaluate(new_c, np, fi) == EvalOk(e.mf.f(fi).outputs[np]))
+      ensures forall np :: np in StateINPs(e.mf.state) ==>
+          np in e.mf.f(fi).state &&
+          NPValid(new_c, np) &&
+          (Evaluate(new_c, np, fi) == EvalOk(e.mf.f(fi).state[np]))
     {
       EntityFOutputsAreValid(c, e1);
       EntityFOutputsAreValid(c, e2);
       FOutputsInSc(c, e1);
       FOutputsInSc(c, e2);
-      reveal EntityFValid();
-      forall np | np in e.foutputs
+      reveal MapFunctionValid();
+      forall np | np in e.mf.outputs
         ensures
-          //e.f.requires(knowns) &&
-          && np in e.f(knowns)
+          && np in e.mf.f(fi).outputs
           && NPValid(new_c, np)
-          && (Evaluate(new_c, np, knowns) == EvalOk(e.f(knowns)[np]))
+          && (Evaluate(new_c, np, fi) == EvalOk(e.mf.f(fi).outputs[np]))
       {
         EntityFOutputsAreValid(new_c, e);
         reveal NPsInSc();
         assert NPValid(new_c, np);
-        EvaluateConnectEntities(c, e1, e2, connection, new_c, np, knowns);
-        assert (Evaluate(new_c, np, knowns) == EvalOk(e.f(knowns)[np]));
+        EvaluateConnectEntities(c, e1, e2, connection, new_c, np, fi);
+        assert (Evaluate(new_c, np, fi) == EvalOk(e.mf.f(fi).outputs[np]));
+      }
+      forall np | np in StateINPs(e.mf.state)
+        ensures
+          && np in e.mf.f(fi).state
+          && NPValid(new_c, np)
+          && (Evaluate(new_c, np, fi) == EvalOk(e.mf.f(fi).state[np]))
+      {
+        EntityFOutputsAreValid(new_c, e);
+        reveal NPsInSc();
+        assert NPValid(new_c, np);
+        EvaluateConnectEntities(c, e1, e2, connection, new_c, np, fi);
+        assert (Evaluate(new_c, np, fi) == EvalOk(e.mf.f(fi).state[np]));
       }
     }
     reveal EntityEvaluatesCorrectly();
@@ -874,9 +937,9 @@ module ConnectionEval {
       reveal ConnectEntitiesImpl();
       reveal ScValid();
     }
-    assert forall knowns: map<NP, bool> :: knowns.Keys == e.finputs ==>
-      forall np :: np in e.foutputs ==>
-        && Evaluate(new_c, np, knowns) == EvalOk(e.f(knowns)[np]);
+    assert forall fi: FI :: FIValid(fi, e.mf.inputs, e.mf.state) ==>
+      forall np :: np in e.mf.outputs ==>
+        && Evaluate(new_c, np, fi) == EvalOk(e.mf.f(fi).outputs[np]);
     assert EntityEvaluatesCorrectly(new_c, e);
     assert EntityValid(new_c, e);
   }
